theories/AutoSubst/core.v
@@ -107,7 +107,7 @@ Defined.
 (* a.d. TODO hints outside of sections without explicit locality are deprecated. Is this even used in the first place?  *)
 (* but with 8.13.1 the attribute is forbidden. So what's the correct way to use this? *)
 (* #[ global ] *)
-#[global]Hint Rewrite in_map_iff : FunctorInstances.
+Hint Rewrite in_map_iff : FunctorInstances.
 
 (* Declaring the scopes that all our notations will live in *)
 Declare Scope fscope.
@@ -140,7 +140,7 @@ Proof.
   trivial.
 Qed.
 
-#[global]Instance funcomp_morphism {X Y Z} :
+Instance funcomp_morphism {X Y Z} :
   Proper (@pointwise_relation Y Z eq ==> @pointwise_relation X Y eq ==> @pointwise_relation X Z eq) funcomp.
 Proof.
   cbv - [funcomp].
@@ -149,7 +149,7 @@ Proof.
   reflexivity.
 Qed.
 
-#[global]Instance funcomp_morphism2 {X Y Z} :
+Instance funcomp_morphism2 {X Y Z} :
   Proper (@pointwise_relation Y Z eq ==> @pointwise_relation X Y eq ==> eq ==> eq) funcomp.
 Proof.
   intros g0 g1 Hg f0 f1 Hf ? x ->.
